

Use ampersand ONLY in an aligned section.
https://tex.stackexchange.com/questions/655/what-is-the-difference-between-def-and-newcommand
https://en.wikibooks.org/wiki/LaTeX/Macros

$$
\newcommand{\alldata}{\space 
  \color{red}{\mathrm{{all{\space}data}} \space }}
\newcommand{\OR}{\space \mathrm{or}\space}
\newcommand{\AND}{\space \mathrm{and}\space}
\newcommand{\RR}{\color{red}{R1 \AND R2}}
$$

$$
\begin{aligned}
Odds(+D|\alldata) & =\frac{Pr(+D|\alldata )}{Pr(-D|\alldata )}\\
& =\frac{Pr(\alldata \AND +D)/Pr(\alldata )}
      {Pr(\alldata \AND -D)/Pr(\alldata )}\\
& = \frac{Pr(\alldata |+D)}{Pr(\alldata |-D)}\ \frac{Pr(+D)}{Pr(-D)}\\
& = LR(\alldata)\times Odds(+D)
\end{aligned}
$$

$$
\begin{aligned}
Odds(+D|\RR) & =\frac{Pr(+D|\RR)}{Pr(-D|\RR)}\\
& =\frac{Pr(\RR \AND +D)\quad/\space Pr(\RR)}
      {Pr(\RR \AND -D)\quad/\space Pr(\RR)}\\
& = \frac{Pr(\RR|+D)}{Pr(\RR|-D)}\ \frac{Pr(+D)}{Pr(-D)}\\
& =LR(\RR)\times Odds(+D)
\end{aligned}
$$

$$
\begin{aligned}
LR(\RR) &= 
\frac{Pr(\RR|+D)}{Pr(\RR|-D)}\\
&= \frac{Pr(R1|+D)Pr(R2|+D)}{Pr(R1|-D)Pr(R2|-D)}\\
&= LR(R1) \times LR(R2)
\end{aligned}
$$

Now, suppose the "prior" says that some KNOWN portion of the true D's are "hidden" (hD) from the test, instead of detectable (dD).
Then the likelihood ratio is now
$$
\begin{aligned}
LR(\RR)
&= 
\frac{Pr(R1 \AND R2 | dD \OR hD)} 
  {Pr(R1 \AND R2|-D)}
\end{aligned}
$$

$$
\begin{aligned}
Pr(R1 \AND R2 | dD \OR hD)
&= 
\frac{Pr(R1 \AND R2 | dD)Pr(dD)+Pr(R1 \AND R2 | hD)Pr(hD)}
{Pr(dD \OR  hD)
}\\
&= 
\frac{Pr(R1 | dD) ^{2} Pr(dD)+Pr(R1 | hD)Pr(hD)}
{Pr(dD) + Pr(hD)
}\\
\end{aligned}
$$
Note that $Pr(R1 | dD) ^{2}$ is squared, because for dD R1 and R2 are conditionally independent. For a dD person, getting the right answer for R1 doesn't increase or decrease th chance of a right answer for R2.

But $Pr(R1 | hD)$ is not squared, because for $hD$, whatever $R1$ is, $R2$ will give the same answer.

For the denominator of the likelihood ratio,
$$
\begin{aligned}
  {Pr(R1 \AND R2|-D)} 
  &= {Pr(R1 |-D)} \times 
  {Pr( R2|-D)}\\
&= {Pr(R1 |-D)} ^{2}
\end{aligned}
$$

because for $-D$, the two reports are conditionally independent. 

